libcrux-iot/sha3/proofs/lean/LibcruxIotSha3/Extraction/Funs.lean
@@ -4688,7 +4688,7 @@ def digest_size (mode : Algorithm) : RustM Std.Usize := do
   | Algorithm.Sha512 => ok SHA3_512_DIGEST_SIZE
 
 /-- [libcrux_iot_sha3::keccakx1]:
-    Source: 'sha3/src/lib.rs', lines 574:0-576:1 -/
+    Source: 'sha3/src/lib.rs', lines 590:0-592:1 -/
 def keccakx1
   (RATE : Std.Usize) (DELIM : Std.U8) (data : Slice Std.U8)
   (out : Slice Std.U8) :
@@ -4697,7 +4697,7 @@ def keccakx1
   keccak.keccak RATE DELIM data out
 
 /-- [libcrux_iot_sha3::sha512_ema]:
-    Source: 'sha3/src/lib.rs', lines 297:0-304:1
+    Source: 'sha3/src/lib.rs', lines 313:0-320:1
     Visibility: public -/
 def sha512_ema
   (digest : Slice Std.U8) (payload : Slice Std.U8) : RustM (Slice Std.U8) := do
@@ -4709,7 +4709,7 @@ def sha512_ema
   keccakx1 72#usize 6#u8 payload digest
 
 /-- [libcrux_iot_sha3::sha384_ema]:
-    Source: 'sha3/src/lib.rs', lines 264:0-271:1
+    Source: 'sha3/src/lib.rs', lines 276:0-283:1
     Visibility: public -/
 def sha384_ema
   (digest : Slice Std.U8) (payload : Slice Std.U8) : RustM (Slice Std.U8) := do
@@ -4721,7 +4721,7 @@ def sha384_ema
   keccakx1 104#usize 6#u8 payload digest
 
 /-- [libcrux_iot_sha3::sha256_ema]:
-    Source: 'sha3/src/lib.rs', lines 231:0-238:1
+    Source: 'sha3/src/lib.rs', lines 239:0-246:1
     Visibility: public -/
 def sha256_ema
   (digest : Slice Std.U8) (payload : Slice Std.U8) : RustM (Slice Std.U8) := do
@@ -4733,7 +4733,7 @@ def sha256_ema
   keccakx1 136#usize 6#u8 payload digest
 
 /-- [libcrux_iot_sha3::sha224_ema]:
-    Source: 'sha3/src/lib.rs', lines 198:0-205:1
+    Source: 'sha3/src/lib.rs', lines 202:0-209:1
     Visibility: public -/
 def sha224_ema
   (digest : Slice Std.U8) (payload : Slice Std.U8) : RustM (Slice Std.U8) := do
@@ -4805,7 +4805,7 @@ def sha224 (payload : Slice Std.U8) : RustM (Array Std.U8 28#usize) := do
   ok (index_mut_back s1)
 
 /-- [libcrux_iot_sha3::sha256]:
-    Source: 'sha3/src/lib.rs', lines 212:0-223:1
+    Source: 'sha3/src/lib.rs', lines 216:0-227:1
     Visibility: public -/
 def sha256 (payload : Slice Std.U8) : RustM (Array Std.U8 32#usize) := do
   let a := Array.repeat 32#usize 0#u8
@@ -4819,7 +4819,7 @@ def sha256 (payload : Slice Std.U8) : RustM (Array Std.U8 32#usize) := do
   ok (index_mut_back s1)
 
 /-- [libcrux_iot_sha3::sha384]:
-    Source: 'sha3/src/lib.rs', lines 245:0-256:1
+    Source: 'sha3/src/lib.rs', lines 253:0-264:1
     Visibility: public -/
 def sha384 (payload : Slice Std.U8) : RustM (Array Std.U8 48#usize) := do
   let a := Array.repeat 48#usize 0#u8
@@ -4833,7 +4833,7 @@ def sha384 (payload : Slice Std.U8) : RustM (Array Std.U8 48#usize) := do
   ok (index_mut_back s1)
 
 /-- [libcrux_iot_sha3::sha512]:
-    Source: 'sha3/src/lib.rs', lines 278:0-289:1
+    Source: 'sha3/src/lib.rs', lines 290:0-301:1
     Visibility: public -/
 def sha512 (payload : Slice Std.U8) : RustM (Array Std.U8 64#usize) := do
   let a := Array.repeat 64#usize 0#u8
@@ -4847,7 +4847,7 @@ def sha512 (payload : Slice Std.U8) : RustM (Array Std.U8 64#usize) := do
   ok (index_mut_back s1)
 
 /-- [libcrux_iot_sha3::shake128]:
-    Source: 'sha3/src/lib.rs', lines 311:0-322:1
+    Source: 'sha3/src/lib.rs', lines 327:0-338:1
     Visibility: public -/
 def shake128
   (BYTES : Std.Usize) (data : Slice Std.U8) : RustM (Array Std.U8 BYTES) := do
@@ -4862,14 +4862,14 @@ def shake128
   ok (index_mut_back s1)
 
 /-- [libcrux_iot_sha3::shake128_ema]:
-    Source: 'sha3/src/lib.rs', lines 331:0-333:1
+    Source: 'sha3/src/lib.rs', lines 347:0-349:1
     Visibility: public -/
 def shake128_ema
   (out : Slice Std.U8) (data : Slice Std.U8) : RustM (Slice Std.U8) := do
   keccakx1 168#usize 31#u8 data out
 
 /-- [libcrux_iot_sha3::shake256]:
-    Source: 'sha3/src/lib.rs', lines 340:0-351:1
+    Source: 'sha3/src/lib.rs', lines 356:0-367:1
     Visibility: public -/
 def shake256
   (BYTES : Std.Usize) (data : Slice Std.U8) : RustM (Array Std.U8 BYTES) := do
@@ -4884,28 +4884,28 @@ def shake256
   ok (index_mut_back s1)
 
 /-- [libcrux_iot_sha3::shake256_ema]:
-    Source: 'sha3/src/lib.rs', lines 360:0-362:1
+    Source: 'sha3/src/lib.rs', lines 376:0-378:1
     Visibility: public -/
 def shake256_ema
   (out : Slice Std.U8) (data : Slice Std.U8) : RustM (Slice Std.U8) := do
   keccakx1 136#usize 31#u8 data out
 
 /-- Trait implementation: [libcrux_iot_sha3::incremental::private::{impl libcrux_iot_sha3::incremental::private::Sealed for libcrux_iot_sha3::incremental::Shake128Xof}]
-    Source: 'sha3/src/lib.rs', lines 387:8-387:45 -/
+    Source: 'sha3/src/lib.rs', lines 403:8-403:45 -/
 @[reducible]
 def incremental.Shake128Xof.Insts.Libcrux_iot_sha3IncrementalPrivateSealed :
   incremental.private.Sealed incremental.Shake128Xof := {
 }
 
 /-- Trait implementation: [libcrux_iot_sha3::incremental::private::{impl libcrux_iot_sha3::incremental::private::Sealed for libcrux_iot_sha3::incremental::Shake256Xof}]
-    Source: 'sha3/src/lib.rs', lines 388:8-388:45 -/
+    Source: 'sha3/src/lib.rs', lines 404:8-404:45 -/
 @[reducible]
 def incremental.Shake256Xof.Insts.Libcrux_iot_sha3IncrementalPrivateSealed :
   incremental.private.Sealed incremental.Shake256Xof := {
 }
 
 /-- [libcrux_iot_sha3::incremental::{impl libcrux_iot_sha3::incremental::Xof<168usize> for libcrux_iot_sha3::incremental::Shake128Xof}::squeeze]:
-    Source: 'sha3/src/lib.rs', lines 468:8-470:9
+    Source: 'sha3/src/lib.rs', lines 484:8-486:9
     Visibility: public -/
 def incremental.Shake128Xof.Insts.Libcrux_iot_sha3IncrementalXof168.squeeze
   (self : incremental.Shake128Xof) (out : Slice Std.U8) :
@@ -4915,7 +4915,7 @@ def incremental.Shake128Xof.Insts.Libcrux_iot_sha3IncrementalXof168.squeeze
   ok ({ state := kxs }, out1)
 
 /-- [libcrux_iot_sha3::incremental::{impl libcrux_iot_sha3::incremental::Xof<168usize> for libcrux_iot_sha3::incremental::Shake128Xof}::absorb_final]:
-    Source: 'sha3/src/lib.rs', lines 464:8-466:9
+    Source: 'sha3/src/lib.rs', lines 480:8-482:9
     Visibility: public -/
 def
   incremental.Shake128Xof.Insts.Libcrux_iot_sha3IncrementalXof168.absorb_final
@@ -4926,7 +4926,7 @@ def
   ok { state := kxs }
 
 /-- [libcrux_iot_sha3::incremental::{impl libcrux_iot_sha3::incremental::Xof<168usize> for libcrux_iot_sha3::incremental::Shake128Xof}::absorb]:
-    Source: 'sha3/src/lib.rs', lines 456:8-458:9
+    Source: 'sha3/src/lib.rs', lines 472:8-474:9
     Visibility: public -/
 def incremental.Shake128Xof.Insts.Libcrux_iot_sha3IncrementalXof168.absorb
   (self : incremental.Shake128Xof) (input : Slice Std.U8) :
@@ -4936,7 +4936,7 @@ def incremental.Shake128Xof.Insts.Libcrux_iot_sha3IncrementalXof168.absorb
   ok { state := kxs }
 
 /-- [libcrux_iot_sha3::incremental::{impl libcrux_iot_sha3::incremental::Xof<168usize> for libcrux_iot_sha3::incremental::Shake128Xof}::new]:
-    Source: 'sha3/src/lib.rs', lines 447:8-451:9
+    Source: 'sha3/src/lib.rs', lines 463:8-467:9
     Visibility: public -/
 def incremental.Shake128Xof.Insts.Libcrux_iot_sha3IncrementalXof168.new
   : RustM incremental.Shake128Xof := do
@@ -4944,7 +4944,7 @@ def incremental.Shake128Xof.Insts.Libcrux_iot_sha3IncrementalXof168.new
   ok { state := kxs }
 
 /-- Trait implementation: [libcrux_iot_sha3::incremental::{impl libcrux_iot_sha3::incremental::Xof<168usize> for libcrux_iot_sha3::incremental::Shake128Xof}]
-    Source: 'sha3/src/lib.rs', lines 446:4-471:5 -/
+    Source: 'sha3/src/lib.rs', lines 462:4-487:5 -/
 @[reducible]
 def incremental.Shake128Xof.Insts.Libcrux_iot_sha3IncrementalXof168 :
   incremental.Xof incremental.Shake128Xof 168#usize := {
@@ -4960,7 +4960,7 @@ def incremental.Shake128Xof.Insts.Libcrux_iot_sha3IncrementalXof168 :
 }
 
 /-- [libcrux_iot_sha3::incremental::{impl libcrux_iot_sha3::incremental::Xof<136usize> for libcrux_iot_sha3::incremental::Shake256Xof}::squeeze]:
-    Source: 'sha3/src/lib.rs', lines 498:8-500:9
+    Source: 'sha3/src/lib.rs', lines 514:8-516:9
     Visibility: public -/
 def incremental.Shake256Xof.Insts.Libcrux_iot_sha3IncrementalXof136.squeeze
   (self : incremental.Shake256Xof) (out : Slice Std.U8) :
@@ -4970,7 +4970,7 @@ def incremental.Shake256Xof.Insts.Libcrux_iot_sha3IncrementalXof136.squeeze
   ok ({ state := kxs }, out1)
 
 /-- [libcrux_iot_sha3::incremental::{impl libcrux_iot_sha3::incremental::Xof<136usize> for libcrux_iot_sha3::incremental::Shake256Xof}::absorb_final]:
-    Source: 'sha3/src/lib.rs', lines 493:8-495:9
+    Source: 'sha3/src/lib.rs', lines 509:8-511:9
     Visibility: public -/
 def
   incremental.Shake256Xof.Insts.Libcrux_iot_sha3IncrementalXof136.absorb_final
@@ -4981,7 +4981,7 @@ def
   ok { state := kxs }
 
 /-- [libcrux_iot_sha3::incremental::{impl libcrux_iot_sha3::incremental::Xof<136usize> for libcrux_iot_sha3::incremental::Shake256Xof}::absorb]:
-    Source: 'sha3/src/lib.rs', lines 485:8-487:9
+    Source: 'sha3/src/lib.rs', lines 501:8-503:9
     Visibility: public -/
 def incremental.Shake256Xof.Insts.Libcrux_iot_sha3IncrementalXof136.absorb
   (self : incremental.Shake256Xof) (input : Slice Std.U8) :
@@ -4991,7 +4991,7 @@ def incremental.Shake256Xof.Insts.Libcrux_iot_sha3IncrementalXof136.absorb
   ok { state := kxs }
 
 /-- [libcrux_iot_sha3::incremental::{impl libcrux_iot_sha3::incremental::Xof<136usize> for libcrux_iot_sha3::incremental::Shake256Xof}::new]:
-    Source: 'sha3/src/lib.rs', lines 475:8-479:9
+    Source: 'sha3/src/lib.rs', lines 491:8-495:9
     Visibility: public -/
 def incremental.Shake256Xof.Insts.Libcrux_iot_sha3IncrementalXof136.new
   : RustM incremental.Shake256Xof := do
@@ -4999,7 +4999,7 @@ def incremental.Shake256Xof.Insts.Libcrux_iot_sha3IncrementalXof136.new
   ok { state := kxs }
 
 /-- Trait implementation: [libcrux_iot_sha3::incremental::{impl libcrux_iot_sha3::incremental::Xof<136usize> for libcrux_iot_sha3::incremental::Shake256Xof}]
-    Source: 'sha3/src/lib.rs', lines 474:4-501:5 -/
+    Source: 'sha3/src/lib.rs', lines 490:4-517:5 -/
 @[reducible]
 def incremental.Shake256Xof.Insts.Libcrux_iot_sha3IncrementalXof136 :
   incremental.Xof incremental.Shake256Xof 136#usize := {
